Prove (forward) type preservation for nnrs->nnrs_imp

coq/Translation/TNNRStoNNRSimp.v
@@ -14,328 +14,739 @@
  * limitations under the License.
  *)
 
-Section TNNRCtoNNRS.
-  Require Import String.
-  Require Import List.
-  Require Import Bool.
-  Require Import Arith.
-  Require Import EquivDec.
-  Require Import Morphisms.
-  Require Import Permutation.
-  Require Import Eqdep_dec.
-  Require Import Program.
-  Require Import Utils.
-  Require Import CommonSystem.
-  Require Import cNNRCSystem.
-  Require Import NNRCSystem.
-  Require Import NNRSSystem.
-  Require Import NNRCtoNNRS.
-  Require Import TNNRCStratify.
+Require Import String.
+Require Import List.
+Require Import Bool.
+Require Import Arith.
+Require Import EquivDec.
+Require Import Morphisms.
+Require Import Permutation.
+Require Import Eqdep_dec.
+Require Import Program.
+Require Import Utils.
+Require Import CommonSystem.
+Require Import NNRSSystem.
+Require Import NNRSimpSystem.
+Require Import NNRStoNNRSimp.
 
-  Local Open Scope nnrs.
+Section TNNRStoNNRSimp.
 
   Context {m:basic_model}.
   Context (τconstants:tbindings).
 
-  Section from_stratified.
+  Definition lift_pdtype (τo:option rtype) : rtype
+    := match τo with
+       | Some τ => τ
+       | None => ⊤
+       end.
+  
+  Definition pd_tbindings_lift (Γ:TNNRS.pd_tbindings) : TNNRSimp.pd_tbindings
+    := map_codomain lift_pdtype Γ.
 
-    Definition pd_tbindings_lift (σ:tbindings) : pd_tbindings
-      := map_codomain Some σ.
-
-    Lemma lookup_pd_tbindings_lift Γ v :
-      lookup equiv_dec (pd_tbindings_lift Γ) v = lift Some (lookup equiv_dec Γ v).
-    Proof.
-      apply lookup_map_codomain.
-    Qed.
-
-    Lemma rproject_eq_preserves_sublist_full
-          {A} {odt:ODT}
-          (l1 l2 : list (string * A)) (sl : list string) :
-      is_list_sorted ODT_lt_dec (domain l1) = true ->
-      is_list_sorted ODT_lt_dec (domain l2) = true ->
-      sublist sl (domain l1) ->
-      rproject l1 sl = rproject l2 sl ->
-      sublist sl (domain l2).
-    Proof.
-      intros.
-      apply Sorted_incl_sublist.
-      - eapply is_list_sorted_Sorted_iff.
-        eapply is_list_sorted_sublist; try eapply H1.
-        eapply H.
-      - eapply is_list_sorted_Sorted_iff; eauto.
-      - intros.
-        assert (inn:In x (domain (rproject l1 sl))).
-        { apply rproject_domain_in; split; trivial.
-          eapply sublist_In; eauto.
-        }
-        rewrite H2 in inn.
-        apply rproject_domain_in in inn; tauto.
-    Qed.
-    
-    Lemma tnnrc_expr_to_nnrs_expr_some_correct {e ei} :
-      nnrc_expr_to_nnrs_expr e = Some ei ->
-      forall (Γc Γ:tbindings) (τ:rtype),
-        nnrc_type Γc Γ e τ <-> [ Γc ; pd_tbindings_lift Γ  ⊢ ei ▷ τ ].
-    Proof.
-      unfold nnrc_type.
-      Hint Constructors nnrc_core_type.
-      Hint Constructors nnrs_expr_type.
-      
-      revert ei.
-      induction e; simpl; intros ei eqq Γc Γ τ; try discriminate.
-      - invcs eqq.
-        split; intros typ; invcs typ; eauto.
-      - invcs eqq.
-        split; intros typ; invcs typ; eauto.
-        + constructor.
-          rewrite lookup_pd_tbindings_lift.
-          rewrite H1; simpl; trivial.
-        + rewrite lookup_pd_tbindings_lift in H1.
-          apply some_lift in H1.
-          destruct H1 as [? ? eqq1]; invcs eqq1.
-          eauto.
-      - invcs eqq; split; intros typ; invcs typ; eauto.
-      - apply some_lift2 in eqq.
-        destruct eqq as [? [??[??]]]; subst.
-        split; intros typ; invcs typ
-        ; (econstructor; eauto 2
-           ; [eapply IHe1 | eapply IHe2]; eauto).        
-      - apply some_lift in eqq.
-        destruct eqq as [? ? ?]; subst.
-        split; intros typ; invcs typ
-        ; (econstructor; eauto 2
-           ; eapply IHe; eauto).        
-      - apply some_lift in eqq.
-        destruct eqq as [? ? ?]; subst.
-        split; intros typ.
-        + change (nnrc_type Γc Γ (NNRCGroupBy s l e) τ) in typ.
-          apply type_NNRCGroupBy_inv in typ.
-          destruct typ as [? [? [? [eqq1 [subl typ]]]]]; subst.
-          constructor; trivial.
-          apply IHe; eauto.
-        +  invcs typ.
-           change (nnrc_type Γc Γ (NNRCGroupBy s l e) (GroupBy_type s l k τl pf)).
-           apply type_NNRCGroupBy; trivial.
-           eapply IHe; eauto.
-    Qed.
-
-    Definition add_term_mc (term:terminator) τ (Δc:mc_tbindings)
-      := match term with
-         | Term_push x => (x,τ)::Δc
-         | Term_assign x => Δc
-         end.
-
-    Definition add_term_md (term:terminator) τ (Δd:md_tbindings)
-      := match term with
-         | Term_push x => Δd
-         | Term_assign x => (x,τ)::Δd
-         end.
-
-    Lemma terminate_type  {Γc:tbindings} {Γ:pd_tbindings} {e τ} :
-      [ Γc ; Γ  ⊢ e ▷ τ ] -> forall term Δc Δd  ,
-        [ Γc ; Γ , (add_term_mc term τ Δc) , (add_term_md term τ Δd) ⊢ terminate term e ].
-    Proof.
-      intros typ term Δc Δd.
-      destruct term; simpl
-      ; econstructor; simpl; try reflexivity; eauto
-      ; match_destr
-      ; congruence.
-    Qed.
-
-    Lemma nnrc_stmt_to_nnrs_stmt_aux_must_assign
-          {fvs x s si} :
-      nnrc_stmt_to_nnrs_stmt_aux fvs (Term_assign x) s = Some si ->
-      nnrs_stmt_must_assign si x.
-    Proof.
-      revert x si.
-      induction s; simpl; intros x si eqq
-      ; repeat match_option_in eqq; invcs eqq; simpl; eauto.
-    Qed.
-    
-    Lemma tnnrc_stmt_to_nnrs_stmt_aux_some_correct_fw {fvs term s si} :
-      nnrc_stmt_to_nnrs_stmt_aux fvs term s = Some si ->
-      forall {Γc:tbindings} {Γ:tbindings} {τ:rtype},
-        nnrc_type Γc Γ s τ ->
-        forall Δc Δd,
-          [ Γc ; pd_tbindings_lift Γ , (add_term_mc term τ Δc) , (add_term_md term τ Δd) ⊢ si ].
-    Proof.
-      unfold nnrc_type.
-      Hint Resolve terminate_type.
-      Hint Constructors nnrc_core_type.
-      Hint Constructors nnrs_expr_type.
-      intros eqq Γc.
-      revert fvs term si eqq.
-      induction s; simpl; intros fvs term si eqq Γ τ typ Δc Δd
-      ; repeat match_option_in eqq; invcs eqq; try solve [invcs typ; eauto 3].
-      - invcs typ.
-        apply terminate_type.
-        econstructor.
-        rewrite lookup_pd_tbindings_lift, H1; simpl; trivial.
-      - apply terminate_type.
-        apply (tnnrc_expr_to_nnrs_expr_some_correct (e:=NNRCBinop b s1 s2))
-        ; simpl; eauto.
-      - apply terminate_type.
-        apply (tnnrc_expr_to_nnrs_expr_some_correct (e:=NNRCUnop u s))
-        ; simpl; eauto.
-      - invcs typ.
-        econstructor.
-        + eapply nnrc_stmt_to_nnrs_stmt_aux_must_assign; eauto.
-        + specialize (IHs1 _ _ _ eqq0 _ _ H4
-                           (add_term_mc term τ Δc)
-                           (add_term_md term τ Δd)); simpl in IHs1; eauto.
-        + specialize (IHs2 _ _ _ eqq1 _ _ H5); simpl in IHs2; eauto.
-      - invcs typ.
-        econstructor.
-        + econstructor.
-          * eapply tnnrc_expr_to_nnrs_expr_some_correct; eauto.
-          * specialize (IHs2 _ _ _ eqq1 _ _ H5); simpl in IHs2; eauto.
-        + apply terminate_type.
-          econstructor; simpl.
-          match_destr; congruence.
-      - invcs typ.
-        econstructor; eauto.
-        apply (tnnrc_expr_to_nnrs_expr_some_correct eqq0); trivial.
-      - invcs typ.
-        econstructor; eauto.
-        + apply (tnnrc_expr_to_nnrs_expr_some_correct eqq0); eauto.
-        + specialize (IHs2 _ _ _ eqq1 _ _ H7); simpl in IHs2; eauto.
-        + specialize (IHs3 _ _ _ eqq2 _ _ H8); simpl in IHs3; eauto.
-      - apply terminate_type.
-        eapply (tnnrc_expr_to_nnrs_expr_some_correct (e:= (NNRCGroupBy s l s0))); simpl; eauto.
-    Qed.
-
-
-    Theorem tnnrc_stmt_to_nnrs_some_correct_fw {Γc:tbindings} {globals s si} :
-      nnrc_stmt_to_nnrs globals s = Some si ->
-      forall {τ:rtype},
-        nnrc_type Γc nil s τ ->
-        [ h, Γc ⊢ si ▷ τ ].
-    Proof.
-      unfold nnrc_stmt_to_nnrs, nnrs_type; match_option
-      ; intros eqq1; invcs eqq1.
-      intros τ typ.
-      unfold nnrc_type in *.
-      apply (tnnrc_stmt_to_nnrs_stmt_aux_some_correct_fw eqq typ).
-    Qed.
-
-    Definition get_terminator_type
-               (term:terminator)
-               (mc:mc_tbindings)
-               (md:md_tbindings) : option rtype :=
-      match term with
-      | Term_assign v => lookup equiv_dec md v
-      | Term_push v => lookup equiv_dec mc v
-      end.
-
-    Lemma terminate_type_inv  {Γc:tbindings} {Γ:pd_tbindings} {e τ} { term Δc Δd }:
-      [ Γc ; Γ , Δc , Δd ⊢ terminate term e ] ->
-      get_terminator_type term Δc Δd = Some τ ->
-      exists τ', [ Γc ; Γ  ⊢ e ▷ τ' ] /\ τ' ≤ τ.
-    Proof.
-      destruct term; simpl; intros typ eqq; invcs typ; simpl in *
-      ; unfold equiv_dec, string_eqdec in *
-      ; rewrite H5 in eqq; invcs eqq
-      ; eauto.
-    Qed.
-
-    Section counterexample.
-      Local Open Scope string.
-      
-      Example nnrc_stmt_with_weaker_nnrs_type_example : nnrc 
-        := NNRCBinop (OpNatBinary NatPlus)
-                     (NNRCConst (dnat 1))
-                     (NNRCConst (dnat 2)).
-
-      Example nnrs_of_nnrc_stmt_with_weaker_nnrs_type_example
-        :=     (NNRSPush "x"
-                            (NNRSBinop (OpNatBinary NatPlus) (NNRSConst (dnat 1))
-                                          (NNRSConst (dnat 2)))).
-
-      Example nnrs_of_nnrc_stmt_with_weaker_nnrs_type_example_correct
-        : nnrc_stmt_to_nnrs_stmt_aux nil (Term_push "x") nnrc_stmt_with_weaker_nnrs_type_example = Some nnrs_of_nnrc_stmt_with_weaker_nnrs_type_example.
-      Proof.
-        vm_compute; reflexivity.
-      Qed.
-
-      Example nnrs_typing_for_nnrc_with_weaker_nnrs_type_example 
-        : [ nil ; pd_tbindings_lift nil , (add_term_mc (Term_push "x") ⊤ nil) , (add_term_md (Term_push "x") ⊤ nil) ⊢ nnrs_of_nnrc_stmt_with_weaker_nnrs_type_example ].
-      Proof.
-        unfold nnrs_of_nnrc_stmt_with_weaker_nnrs_type_example.
-        simpl.
-        econstructor; simpl.
-        - repeat econstructor.
-        - reflexivity.
-        - apply STop.
-      Qed.
-
-      Example nnrc_typing_for_nnrc_with_weaker_nnrs_type_example 
-        : nnrc_type nil nil nnrc_stmt_with_weaker_nnrs_type_example Nat.
-      Proof.
-        unfold nnrc_type, nnrc_stmt_with_weaker_nnrs_type_example.
-        simpl.
-        econstructor; simpl
-        ; repeat econstructor.
-      Qed.
-
-      Example not_nnrc_typing_for_nnrc_with_weaker_nnrs_type_example 
-        : ~ nnrc_type nil nil nnrc_stmt_with_weaker_nnrs_type_example ⊤.
-      Proof.
-        unfold nnrc_type, nnrc_stmt_with_weaker_nnrs_type_example
-        ; simpl; intros typ.
-        invcs typ.
-        invcs H3.
-      Qed.
-
-      Example nnrc_typing_weaker_nnrs_translated_typing :
-        nnrc_stmt_to_nnrs_stmt_aux nil (Term_push "x")
-                                       nnrc_stmt_with_weaker_nnrs_type_example =
-        Some nnrs_of_nnrc_stmt_with_weaker_nnrs_type_example
-        /\ 
-        [ nil ; pd_tbindings_lift nil , (add_term_mc (Term_push "x") ⊤ nil) , (add_term_md (Term_push "x") ⊤ nil)
-                                                                                ⊢ nnrs_of_nnrc_stmt_with_weaker_nnrs_type_example ]
-        /\ ~ nnrc_type nil nil nnrc_stmt_with_weaker_nnrs_type_example ⊤.
-      Proof.
-        split; [ | split].
-        - apply nnrs_of_nnrc_stmt_with_weaker_nnrs_type_example_correct.
-        - apply nnrs_typing_for_nnrc_with_weaker_nnrs_type_example.
-        - apply not_nnrc_typing_for_nnrc_with_weaker_nnrs_type_example.
-      Qed.
-
-    (*
-    Example nnrc_with_weaker_nnrs_type_example : nnrc 
-      := NNRCFor "x"%string (NNRCConst (dcoll (dnat 3:: dnat 4::dnat 5::nil)))
-                 nnrc_stmt_with_weaker_nnrs_type_example.
-     *)
-
-    (* Backwards is more problematic, since the type system for nnrs allows for 
-       free upcasts in a NNRSPush, whereas NNRC typing does not have
-       such a mechanism (and NNRC is not Proper with respect to subtyping, since
-       operators (such as (OpNatBinary NatPlus) are not.
-       For example, 
-       nnrc_typing_weaker_nnrs_translated_typing witnesses a counter example.      *)
-    End counterexample.
-
-  End from_stratified.
-
-  Lemma tnnrc_stmt_to_nnrs_stmt_stratified_some_correct_fw {Γc:tbindings} {globals s τ} :
-    nnrc_type Γc nil s τ ->
-    forall pf,
-      [ h, Γc ⊢ ` (nnrc_stmt_to_nnrs_stmt_stratified_some globals s pf) ▷ τ ].
+  Lemma lookup_pd_tbindings_lift Γ v :
+    lookup equiv_dec (pd_tbindings_lift Γ) v = lift lift_pdtype (lookup equiv_dec Γ v).
   Proof.
-    intros typ pf.
-    destruct (nnrc_stmt_to_nnrs_stmt_stratified_some globals s pf); simpl.
-    eapply tnnrc_stmt_to_nnrs_some_correct_fw; eauto.
+    apply lookup_map_codomain.
+  Qed.
+
+  Lemma tnnrs_expr_to_nnrs_expr_correct_f:
+    forall Γc Γ (e:nnrs_expr) (τ:rtype),
+      ([ Γc ; Γ  ⊢ e ▷ τ ])%nnrs_scope -> [ Γc ; pd_tbindings_lift Γ  ⊢ (nnrs_expr_to_nnrs_imp_expr e) ▷ τ ]%nnrs_imp_scope.
+  Proof.
+    Hint Constructors nnrs_imp_expr_type.
+    intros Γc Γ e.
+    revert Γ.
+    induction e
+    ; simpl
+    ; intros Γ τ typ
+    ; invcs typ
+    ; econstructor; eauto.
+    - rewrite lookup_pd_tbindings_lift.
+      rewrite H1.
+      simpl; trivial.
+  Qed.
+
+  Lemma tnnrs_expr_to_nnrs_expr_correct_b:
+    forall Γc Γ (e:nnrs_expr) (τ:rtype),
+      (forall x, In x (nnrs_expr_free_vars e) -> lookup equiv_dec Γ x <> Some None) ->
+      [ Γc ; pd_tbindings_lift Γ  ⊢ (nnrs_expr_to_nnrs_imp_expr e) ▷ τ ]%nnrs_imp_scope -> ([ Γc ; Γ  ⊢ e ▷ τ ])%nnrs_scope.
+  Proof.
+    Hint Constructors nnrs_expr_type.
+    intros Γc Γ e.
+    revert Γ.
+    induction e
+    ; simpl
+    ; intros Γ τ fns typ
+    ; invcs typ
+    ; econstructor; eauto.
+    - rewrite lookup_pd_tbindings_lift in H1.
+      apply some_lift in H1.
+      destruct H1 as [???]; subst.
+      specialize (fns v); unfold var in *.
+      rewrite e in *.
+      destruct x; simpl; intuition.
+    - eapply IHe1; trivial.
+      intros; apply fns.
+      rewrite in_app_iff; intuition.
+    - eapply IHe2; trivial.
+      intros; apply fns.
+      rewrite in_app_iff; intuition.
   Qed.
   
-  Theorem tnnrc_to_nnrs_correct_fw {Γc:tbindings} {globals s τ} :
-    nnrc_type Γc nil s τ ->
-    [ h, Γc ⊢ (nnrc_to_nnrs_top globals s) ▷ τ ].
+  Definition concat_tenvs
+             (Γ :TNNRS.pd_tbindings)
+             (Δc :TNNRS.mc_tbindings)
+             (Δd :TNNRS.md_tbindings)
+    : TNNRSimp.pd_tbindings
+    := pd_tbindings_lift Γ ++ map_codomain Coll Δc ++ Δd.
+
+  Lemma concat_tenvs_cons (Γ :TNNRS.pd_tbindings)
+        (Δc :TNNRS.mc_tbindings)
+        (Δd :TNNRS.md_tbindings) s τ :
+    (s,lift_pdtype τ)::concat_tenvs Γ Δc Δd = concat_tenvs ((s,τ)::Γ) Δc Δd.
   Proof.
-    intros typ.
-    unfold nnrc_to_nnrs_top.
-    apply tnnrc_stmt_to_nnrs_stmt_stratified_some_correct_fw.
-    apply -> stratify_preserves_types.
-    trivial.
+    reflexivity.
   Qed.
 
-End TNNRCtoNNRS.
+  Lemma concat_tenvs_cons_some (Γ :TNNRS.pd_tbindings)
+        (Δc :TNNRS.mc_tbindings)
+        (Δd :TNNRS.md_tbindings) s τ :
+    (s, τ)::concat_tenvs Γ Δc Δd = concat_tenvs ((s,Some τ)::Γ) Δc Δd.
+  Proof.
+    reflexivity.
+  Qed.
+
+  Lemma concat_tenvs_cons_none (Γ :TNNRS.pd_tbindings)
+        (Δc :TNNRS.mc_tbindings)
+        (Δd :TNNRS.md_tbindings) s  :
+    (s, ⊤)::concat_tenvs Γ Δc Δd = concat_tenvs ((s,None)::Γ) Δc Δd.
+  Proof.
+    reflexivity.
+  Qed.
+
+  (* Move this to TNNRS *)
+  Lemma nnrs_expr_type_lookup_on_equiv {Γc Γ₁ e τ} :
+    ([ Γc ; Γ₁  ⊢ e ▷ τ ])%nnrs_scope ->
+    forall Γ₂,
+      lookup_equiv_on (nnrs_expr_free_vars e) Γ₁ Γ₂ ->
+      ([ Γc ; Γ₂  ⊢ e ▷ τ ])%nnrs_scope.
+  Proof.
+    revert Γ₁ τ.
+    induction e; intros Γ₁ τ typ Γ₂ leo
+    ; invcs typ; simpl in *; subst; econstructor; eauto 3.
+    - rewrite <- leo; simpl; tauto.
+    - eapply IHe1; eauto.
+      unfold lookup_equiv_on in *; intuition.
+    - eapply IHe2; eauto.
+      unfold lookup_equiv_on in *; intuition.
+  Qed.
+
+  Lemma nnrs_expr_to_nnrs_imp_expr_free_vars (e:nnrs_expr) :
+    nnrs_imp_expr_free_vars (nnrs_expr_to_nnrs_imp_expr e) = nnrs_expr_free_vars e.
+  Proof.
+    induction e; simpl; congruence.
+  Qed.
+
+  Lemma nnrs_stmt_to_nnrs_imp_stmt_not_used_without_assignment s v:
+    ~ In v (nnrs_stmt_free_env_vars s) ->
+    ~ In v (nnrs_stmt_free_mcenv_vars s) ->
+    nnrs_imp_stmt_var_usage (nnrs_stmt_to_nnrs_imp_stmt s) v <> VarMayBeUsedWithoutAssignment.
+  Proof.
+    nnrs_stmt_cases (induction s) Case
+    ; simpl
+    ; repeat rewrite in_app_iff
+    ; intros nin1 nin2.
+    - Case "NNRSSeq"%string.
+      match_destr; intuition.
+    - Case "NNRSLet"%string.
+      match_case; intros eqq.
+      + rewrite nnrs_imp_expr_may_use_free_vars in eqq.
+        rewrite nnrs_expr_to_nnrs_imp_expr_free_vars in eqq.
+        tauto.
+      + unfold equiv_decb. destruct (v0 == v); try congruence.
+        apply IHs; try tauto.
+        rewrite remove_in_neq by eauto.
+        tauto.
+    - Case "NNRSLetMut"%string.
+      unfold equiv_decb.
+      destruct (v0 == v); try congruence.
+      match_destr; try tauto.
+      apply IHs2; try tauto.
+      rewrite remove_in_neq by eauto.
+      tauto.
+    - Case "NNRSLetMutColl"%string.
+      unfold equiv_decb.
+      destruct (v0 == v); try congruence.
+      match_destr; try tauto.
+      + elim IHs1; try tauto.
+        rewrite remove_in_neq by eauto.
+        tauto.      
+      + apply IHs2; try tauto.
+        rewrite remove_in_neq by eauto.
+        tauto.      
+    - Case "NNRSAssign"%string.
+      match_case; intros eqq.
+      + rewrite nnrs_imp_expr_may_use_free_vars in eqq.
+        rewrite nnrs_expr_to_nnrs_imp_expr_free_vars in eqq.
+        tauto.
+      + match_destr.
+    - Case "NNRSPush"%string.
+      unfold equiv_decb.
+      destruct (v == v0); destruct (v0 == v); try congruence; simpl.
+      + tauto.
+      + match_case; intros eqq.
+        rewrite nnrs_imp_expr_may_use_free_vars in eqq.
+        rewrite nnrs_expr_to_nnrs_imp_expr_free_vars in eqq.
+        tauto.
+    - Case "NNRSFor"%string.
+      match_case; intros eqq.
+      + rewrite nnrs_imp_expr_may_use_free_vars in eqq.
+        rewrite nnrs_expr_to_nnrs_imp_expr_free_vars in eqq.
+        tauto.
+      + unfold equiv_decb. destruct (v0 == v); try congruence.
+        match_case; intros eqq2.
+        elim IHs; try tauto.
+        rewrite remove_in_neq by eauto.
+        tauto.
+    - Case "NNRSIf"%string.
+      match_case; intros eqq.
+      + rewrite nnrs_imp_expr_may_use_free_vars in eqq.
+        rewrite nnrs_expr_to_nnrs_imp_expr_free_vars in eqq.
+        tauto.
+      + match_case; intros eqq2
+        ; try (match_case; intros eqq3).
+        * elim IHs2; try tauto.
+        * elim IHs1; try tauto.
+        * elim IHs2; try tauto.
+    - Case "NNRSEither"%string.
+      match_case; intros eqq.
+      + rewrite nnrs_imp_expr_may_use_free_vars in eqq.
+        rewrite nnrs_expr_to_nnrs_imp_expr_free_vars in eqq.
+        tauto.
+      + destruct (v0 == v).
+        * destruct (v1 == v); try congruence.
+          match_case; intros eqq2.
+          elim IHs2; try tauto.
+          rewrite remove_in_neq by eauto.
+          tauto.
+        * { match_case; intros eqq2.
+            - destruct (v1 == v); try congruence.
+              match_case; intros eqq3.
+              elim IHs2; try tauto.
+              rewrite remove_in_neq by eauto.
+              tauto.
+            - elim IHs1; try tauto.
+              rewrite remove_in_neq by eauto.
+              tauto.
+            - destruct (v1 == v); try congruence.
+              match_case; intros eqq3.
+              elim IHs2; try tauto.
+              rewrite remove_in_neq by eauto.
+              tauto.
+          }
+  Qed.
+
+  Lemma nnrs_imp_stmt_free_used s x :
+    nnrs_imp_stmt_var_usage s x <> VarNotUsedAndNotAssigned ->
+    In x (nnrs_imp_stmt_free_vars s).
+  Proof.
+    nnrs_imp_stmt_cases (induction s) Case
+    ; simpl
+    ; repeat rewrite in_app_iff
+    ; try rewrite nnrs_imp_expr_may_use_free_vars
+    ; try rewrite IHs
+    ; try rewrite IHs1
+    ; try rewrite IHs2.
+    - Case "NNRSimpSeq"%string.
+      match_case; intuition congruence.
+    - Case "NNRSimpAssign"%string.
+      match_case; try congruence
+      ; try rewrite nnrs_imp_expr_may_use_free_vars
+      ; try rewrite nnrs_imp_expr_may_use_free_vars_neg.
+      + intuition congruence.
+      + unfold equiv_decb; destruct (v == x); intuition congruence.
+    - Case "NNRSimpLet"%string.
+      destruct o.
+      + (match_case; intros eqq)
+        ; try rewrite nnrs_imp_expr_may_use_free_vars in eqq
+        ; try rewrite nnrs_imp_expr_may_use_free_vars_neg in eqq.
+        * intuition congruence.
+        * { unfold equiv_decb; destruct (v == x); unfold equiv, complement in *.
+            - subst.
+              intuition.
+            - intuition.
+              right; apply remove_in_neq; intuition.
+          }
+      + simpl; intuition.
+        unfold equiv_decb in *; destruct (v ==x); try intuition congruence.
+        right.
+        apply remove_in_neq; intuition.
+    - Case "NNRSimpFor"%string.
+      (match_case; intros eqq)
+      ; try rewrite nnrs_imp_expr_may_use_free_vars in eqq
+      ; try rewrite nnrs_imp_expr_may_use_free_vars_neg in eqq.
+      + intuition congruence.
+      +  unfold equiv_decb; destruct (v == x); unfold equiv, complement in *.
+         * subst.
+           intuition.
+         * { match_case; intros eqq2; try congruence.
+             rewrite <- remove_in_neq by eauto.
+             right; apply IHs.
+             intuition; try congruence.
+           }
+    - Case "NNRSimpIf"%string.
+      (match_case; intros eqq)
+      ; try rewrite nnrs_imp_expr_may_use_free_vars in eqq
+      ; try rewrite nnrs_imp_expr_may_use_free_vars_neg in eqq.
+      + intuition congruence.
+      + match_case; intros eqq1
+        ; try (match_case; intros eqq2)
+        ; try intuition congruence.
+    - Case "NNRSimpEither"%string.
+      (match_case; intros eqq)
+      ; try rewrite nnrs_imp_expr_may_use_free_vars in eqq
+      ; try rewrite nnrs_imp_expr_may_use_free_vars_neg in eqq.
+      + intuition congruence.
+      + destruct (v == x).
+        * { destruct (v0 == x)
+            ; try intuition congruence.
+            match_case; intros eqq1
+            ; try (match_case; intros eqq2)
+            ; try intuition congruence.
+            right; right.
+            rewrite <- remove_in_neq by eauto.
+            apply IHs2; congruence.
+          } 
+        * { match_case; intros eqq1.
+            -  destruct (v0 == x)
+               ; try intuition congruence.
+               match_case; intros eqq2
+               ; try intuition congruence.
+               + right; left.
+                 rewrite <- remove_in_neq by eauto.
+                 apply IHs1; congruence.
+               + right; left.
+                 rewrite <- remove_in_neq by eauto.
+                 apply IHs1; congruence.
+            -  right; left.
+               rewrite <- remove_in_neq by eauto.
+               apply IHs1; congruence.
+            - destruct (v0 == x)
+              ; try intuition congruence.
+              match_case; intros eqq2
+              ; try intuition congruence.
+              + right; right.
+                rewrite <- remove_in_neq by eauto.
+                apply IHs2; congruence.
+          }
+  Qed.
+
+  Lemma nnrs_stmt_to_nnrs_imp_stmt_must_assign_assigned {s dΓ dΔc dΔd} :
+    nnrs_stmt_cross_shadow_free_under s dΓ dΔc dΔd ->
+    forall v,
+      In v (dΔd) ->
+      nnrs_stmt_must_assign s v ->
+      nnrs_imp_stmt_var_usage (nnrs_stmt_to_nnrs_imp_stmt s) v = VarMustBeAssigned.
+  Proof.
+    revert dΓ dΔc dΔd.
+    nnrs_stmt_cases (induction s) Case
+    ; simpl
+    ; repeat rewrite in_app_iff
+    ; intros dΓ dΔc dΔd cs vv inn ma.
+    - Case "NNRSSeq"%string.
+      specialize (IHs1 dΓ dΔc dΔd).
+      specialize (IHs2 dΓ dΔc dΔd).
+      (match_case; intro); intuition
+      ; try solve[(eelim (nnrs_stmt_to_nnrs_imp_stmt_not_used_without_assignment)
+                   ; [| | eauto]; eauto)]
+      ; try congruence.
+      + rewrite H3 in H; intuition.
+      + eelim nnrs_stmt_to_nnrs_imp_stmt_not_used_without_assignment; [| | eauto]; eauto.
+        * apply nnrs_stmt_cross_shadow_free_under_free_env_mdenv in H0.
+          specialize (H0 vv); tauto.
+        * apply nnrs_stmt_cross_shadow_free_under_free_mcenv_mdenv in H0.
+          specialize (H0 vv); tauto.
+      + rewrite H3 in H; congruence.
+    - Case "NNRSLet"%string.
+      match_case; intros eqq
+      ; try rewrite nnrs_imp_expr_may_use_free_vars in eqq
+      ; try rewrite nnrs_imp_expr_may_use_free_vars_neg in eqq
+      ; try rewrite nnrs_expr_to_nnrs_imp_expr_free_vars in eqq
+      ; intuition.
+      + specialize (H1 vv); intuition.
+      + unfold equiv_decb; destruct (v == vv); unfold equiv, complement in *
+        ; subst
+        ; intuition; eauto.
+    - Case "NNRSLetMut"%string.
+      unfold equiv_decb; destruct (v == vv); unfold equiv, complement in *
+      ; subst
+      ; intuition.
+      + rewrite (IHs1 _ _ _  H2 vv); simpl; tauto.
+      + match_case; intros eqq.
+        * { eelim nnrs_stmt_to_nnrs_imp_stmt_not_used_without_assignment; [| | eauto]; eauto.
+            - apply nnrs_stmt_cross_shadow_free_under_free_env_mdenv in H2.
+              specialize (H2 vv); simpl in H2; tauto.
+            - apply nnrs_stmt_cross_shadow_free_under_free_mcenv_mdenv in H2.
+              specialize (H2 vv); simpl in H2; tauto.
+          }
+        * eauto.
+    - Case "NNRSLetMutColl"%string.
+      unfold equiv_decb; destruct (v == vv); unfold equiv, complement in *
+      ; subst
+      ; intuition.
+      + rewrite (IHs1 _ _ _  H2 vv); simpl; tauto.
+      + match_case; intros eqq.
+        * { eelim nnrs_stmt_to_nnrs_imp_stmt_not_used_without_assignment; [| | eauto]; eauto.
+            - apply nnrs_stmt_cross_shadow_free_under_free_env_mdenv in H2.
+              specialize (H2 vv); simpl in H2; tauto.
+            - apply nnrs_stmt_cross_shadow_free_under_free_mcenv_mdenv in H2.
+              specialize (H2 vv); simpl in H2; tauto.
+          }
+        * eauto.        
+    - Case "NNRSAssign"%string.
+      subst.
+      match_case; intros eqq.
+      + rewrite nnrs_imp_expr_may_use_free_vars in eqq.
+        rewrite nnrs_expr_to_nnrs_imp_expr_free_vars in eqq.
+        subst; intuition.
+        specialize (H1 vv); tauto.
+      + unfold equiv_decb; destruct (vv == vv); try congruence.
+    - Case "NNRSPush"%string.
+      contradiction.
+    - Case "NNRSFor"%string.
+      match_case; intros eqq
+      ; try rewrite nnrs_imp_expr_may_use_free_vars in eqq
+      ; try rewrite nnrs_imp_expr_may_use_free_vars_neg in eqq
+      ; try rewrite nnrs_expr_to_nnrs_imp_expr_free_vars in eqq
+      ; intuition.
+    - Case "NNRSIf"%string.
+      match_case; intros eqq
+      ; try rewrite nnrs_imp_expr_may_use_free_vars in eqq
+      ; try rewrite nnrs_imp_expr_may_use_free_vars_neg in eqq
+      ; try rewrite nnrs_expr_to_nnrs_imp_expr_free_vars in eqq
+      ; intuition.
+      + specialize (H3 vv); tauto.
+      + rewrite (IHs1 _ _ _ H0); trivial.
+        rewrite (IHs2 _ _ _ H5); trivial.
+    - Case "NNRSEither"%string.
+      match_case; intros eqq
+      ; try rewrite nnrs_imp_expr_may_use_free_vars in eqq
+      ; try rewrite nnrs_imp_expr_may_use_free_vars_neg in eqq
+      ; try rewrite nnrs_expr_to_nnrs_imp_expr_free_vars in eqq
+      ; intuition.
+      + specialize (H3 vv); tauto.
+      + specialize (IHs1 _ _ _ H7 _ inn H1).
+        specialize (IHs2 _ _ _ H9 _ inn H2).
+        rewrite IHs1, IHs2.
+        destruct (v == vv); try congruence.
+        destruct (v0 == vv); try congruence.
+  Qed.
+
+  Lemma concat_tenvs_lookup_equiv_env_mc_cons Γ Δc Δd v τ :
+    ~ In v (domain Γ) ->
+    lookup_equiv (concat_tenvs ((v,Some (Coll τ))::Γ) Δc Δd)
+                 (concat_tenvs Γ ((v,τ)::Δc) Δd).
+  Proof.
+    unfold concat_tenvs, lookup_equiv.
+    intros nin x.
+    repeat rewrite lookup_app; simpl.
+    destruct (string_eqdec x v); unfold equiv, complement in *.
+    + subst. rewrite lookup_nin_none; trivial.
+      unfold pd_tbindings_lift.
+      rewrite domain_map_codomain; trivial.
+    + trivial.
+  Qed.
+
+  Lemma concat_tenvs_lookup_equiv_mc_md  Γ Δc Δd v τ :
+    ~ In v (domain Δc) ->
+    lookup_equiv (concat_tenvs Γ ((v,τ)::Δc) Δd)
+                 (concat_tenvs Γ Δc ((v,Coll τ)::Δd)).
+  Proof.
+    unfold concat_tenvs, lookup_equiv.
+    intros nin x.
+    repeat rewrite lookup_app.
+    match_destr; simpl.
+    destruct (string_eqdec x v); unfold equiv, complement in *.
+    + subst.
+      rewrite lookup_nin_none; trivial.
+      rewrite domain_map_codomain; trivial.
+    + match_destr.
+  Qed.
+
+  Lemma concat_tenvs_lookup_equiv_env_md Γ Δc Δd v τ :
+    ~ In v (domain Γ) ->
+    ~ In v (domain Δc) ->
+    lookup_equiv (concat_tenvs ((v,τ)::Γ) Δc Δd)
+                 (concat_tenvs Γ Δc ((v,lift_pdtype τ)::Δd)).
+  Proof.
+    intros nin1 nin2 x.
+    unfold concat_tenvs, lookup_equiv.
+    repeat rewrite lookup_app; simpl.
+    destruct (string_eqdec x v); unfold equiv, complement in *.
+    + subst.
+      repeat rewrite lookup_nin_none; trivial
+      ; unfold pd_tbindings_lift; rewrite domain_map_codomain; trivial.
+    + trivial.
+  Qed.
+  
+  Lemma nnrs_stmt_unused_tenv_free_env {Γc Γ Δc Δd s} :
+    [ Γc ; Γ , Δc , Δd ⊢ s ]%nnrs_scope ->
+    forall x, 
+      lookup equiv_dec Γ x = Some None ->
+      ~ In x (nnrs_stmt_free_env_vars s).
+  Proof.
+    revert Γ Δc Δd.
+    nnrs_stmt_cases (induction s) Case
+    ; simpl; intros Γ Δc Δd typ x eqq
+    ; invcs typ
+    ; repeat rewrite in_app_iff.
+    - Case "NNRSSeq"%string.
+      intuition eauto.
+    - Case "NNRSLet"%string.
+      intuition eauto.
+      + eapply nnrs_expr_unused_tenv_free_env; eauto.
+      + apply remove_inv in H0.
+        intuition.
+        eapply IHs; eauto; simpl.
+        match_destr; congruence.
+    - Case "NNRSLetMut"%string.
+      intuition.
+      + eapply IHs1; eauto.
+      + apply remove_inv in H0; intuition.
+        eapply IHs2; eauto.
+        simpl; match_destr; congruence.
+    - Case "NNRSLetMut"%string.
+      intuition.
+      + eapply IHs1; eauto.
+      + apply remove_inv in H0; intuition.
+        eapply IHs2; eauto.
+        simpl; match_destr; congruence.
+    - Case "NNRSLetMutColl"%string.
+      intuition.
+      + eapply IHs1; eauto.
+      + apply remove_inv in H0; intuition.
+        eapply IHs2; eauto.
+        simpl; match_destr; congruence.
+    - Case "NNRSAssign"%string.
+      eapply nnrs_expr_unused_tenv_free_env; eauto.
+    - Case "NNRSPush"%string.
+      eapply nnrs_expr_unused_tenv_free_env; eauto.
+    - Case "NNRSFor"%string.
+      intuition eauto.
+      + apply (nnrs_expr_unused_tenv_free_env H4) in eqq; tauto.
+      + apply remove_inv in H0.
+        intuition.
+        eapply IHs; eauto; simpl.
+        match_destr; congruence.
+    - Case "NNRSIf"%string.
+      intuition eauto.
+      eapply nnrs_expr_unused_tenv_free_env; eauto.
+    - Case "NNRSEither"%string.
+      intuition eauto.
+      + eapply nnrs_expr_unused_tenv_free_env; eauto.
+      + apply remove_inv in H.
+        intuition.
+        eapply IHs1; eauto; simpl.
+        match_destr; congruence.
+      + apply remove_inv in H.
+        intuition.
+        eapply IHs2; eauto; simpl.
+        match_destr; congruence.
+  Qed.
+
+  Lemma tnnrs_stmt_to_nnrs_imp_correct_f
+        {Γc:tbindings} {Γ:TNNRS.pd_tbindings}
+        (Δc:TNNRS.mc_tbindings) (Δd:TNNRS.md_tbindings) s :
+    [ Γc ; Γ , Δc , Δd ⊢ s ]%nnrs_scope ->
+    nnrs_stmt_cross_shadow_free_under s (domain Γ) (domain Δc) (domain Δd)->
+    [ Γc ; concat_tenvs Γ Δc Δd ⊢  nnrs_stmt_to_nnrs_imp_stmt s ]%nnrs_imp_scope.
+  Proof.
+
+    Ltac prove_expr_f_t
+         := match goal with
+            | [H: [ _ ; _ ⊢ ?e ▷ _ ]%nnrs_scope |-
+               [ _ ; _ ⊢ nnrs_expr_to_nnrs_imp_expr ?e ▷ _ ] %nnrs_imp_scope ] =>
+              apply tnnrs_expr_to_nnrs_expr_correct_f in H
+              ; apply (nnrs_imp_expr_type_lookup_on_equiv H)
+              ; rewrite nnrs_expr_to_nnrs_imp_expr_free_vars
+              ; unfold lookup_equiv_on; intros ? inn
+              ; unfold concat_tenvs; repeat rewrite lookup_app
+              ; match_destr
+              ; repeat rewrite lookup_nin_none; trivial
+              ; try rewrite domain_map_codomain; trivial
+              ; match goal with
+                | [H1:disjoint ?l1 ?l2,
+                      H2: In ?x ?l1 |- ~ In ?x ?l2 ] =>
+                  exact (H1 x inn)
+                end
+            end.
+    
+    Hint Constructors nnrs_imp_stmt_type.
+    revert Γ Δc Δd.
+    nnrs_stmt_cases (induction s) Case
+    ; simpl; intros Γ Δc Δd typ sf
+    ; invcs typ.
+    - Case "NNRSSeq"%string.
+      econstructor; intuition eauto.
+    - Case "NNRSLet"%string.
+      destruct sf as [disj1 [disj2 [nin1 [nin2 sf]]]].
+      econstructor.
+      + prove_expr_f_t.
+      + specialize (IHs ((v, Some τ) :: Γ)); unfold concat_tenvs in *.
+        simpl in IHs; eauto.
+    - Case "NNRSLetMut"%string.
+      destruct sf as [ninΓ [ninΔc [ninΔd [sf1 sf2]]]].
+      apply (nnrs_stmt_to_nnrs_imp_stmt_must_assign_assigned sf1) in H5
+      ; simpl; try tauto.
+      eapply (type_NNRSimpLetNone _ _ τ); simpl.
+      + rewrite H5; congruence.
+      + specialize (IHs1 _ _ _ H6 sf1).
+        specialize (IHs2 _ _ _ H7 sf2).
+        econstructor.
+        * eapply nnrs_imp_stmt_type_lookup_equiv_prop; eauto.
+          rewrite concat_tenvs_cons_some.
+          apply concat_tenvs_lookup_equiv_env_md; eauto.
+        * eauto.
+    - Case "NNRSLetMut"%string.
+      destruct sf as [ninΓ [ninΔc [ninΔd [sf1 sf2]]]].
+      eapply (type_NNRSimpLetNone _ _ ⊤); simpl.
+      + match_case; intros eqq; try congruence.
+        * { apply nnrs_stmt_to_nnrs_imp_stmt_not_used_without_assignment in eqq.
+            - contradiction.
+            - apply nnrs_stmt_cross_shadow_free_under_free_env_mdenv in sf1.
+              specialize (sf1 v); simpl in sf1; tauto.
+            - apply nnrs_stmt_cross_shadow_free_under_free_mcenv_mdenv in sf1.
+              specialize (sf1 v); simpl in sf1; tauto.
+          }
+        * { apply nnrs_stmt_to_nnrs_imp_stmt_not_used_without_assignment.
+            - apply (nnrs_stmt_unused_tenv_free_env H6 v); simpl.
+              match_destr; try congruence.
+            - apply nnrs_stmt_cross_shadow_free_under_free_mcenv_env in sf2.
+              eapply disjoint_cons_inv2 in sf2; tauto.
+          }
+      + rewrite concat_tenvs_cons_none.
+        econstructor; eauto.
+        eapply nnrs_imp_stmt_type_lookup_equiv_prop; eauto.
+        apply concat_tenvs_lookup_equiv_env_md; eauto.
+    - Case "NNRSLetMutColl"%string.
+      destruct sf as [ninΓ [ninΔc [ninΔd [sf1 sf2]]]].
+      eapply (type_NNRSimpLetDef _ _ (Coll τ)); simpl.
+      + repeat (econstructor; simpl).
+      + rewrite concat_tenvs_cons_some.
+        econstructor; eauto.
+        eapply nnrs_imp_stmt_type_lookup_equiv_prop; eauto.
+        apply concat_tenvs_lookup_equiv_env_mc_cons; eauto.
+    - Case "NNRSAssign"%string.
+      destruct sf as [disjc [disjd [ninΓ ninΔc]]].
+      econstructor; eauto.
+      + prove_expr_f_t. 
+      + unfold concat_tenvs; repeat rewrite lookup_app.
+        rewrite H5.
+        repeat rewrite lookup_nin_none; trivial
+        ; unfold pd_tbindings_lift
+        ; try rewrite domain_map_codomain; trivial.
+      + reflexivity.
+    - Case "NNRSPush"%string.
+      destruct sf as [disjc [disjd [ninΓ ninΔc]]].
+      assert (lo:lookup equiv_dec (concat_tenvs Γ Δc Δd) v = Some (Coll τ)).
+      {
+        unfold concat_tenvs; repeat rewrite lookup_app.
+        rewrite lookup_map_codomain.
+        unfold equiv_dec, string_eqdec.
+        rewrite H5.
+        repeat rewrite lookup_nin_none; trivial
+        ; unfold pd_tbindings_lift
+        ; try rewrite domain_map_codomain; trivial.
+      } 
+      econstructor; eauto; [| eapply SColl; eauto; reflexivity].
+      econstructor; eauto; [econstructor | ].
+      econstructor; [econstructor | ].
+      prove_expr_f_t.
+    - Case "NNRSFor"%string.
+      destruct sf as [disjc [disjd [ninΔc [ninΔd sf]]]].
+      econstructor.
+      + prove_expr_f_t.
+      + specialize (IHs ((v, Some τ) :: Γ)); unfold concat_tenvs in *.
+         simpl in IHs; eauto.
+    - Case "NNRSIf"%string.
+      destruct sf as [disjc [disjd [sf1 sf2]]].
+      econstructor; eauto.
+      prove_expr_f_t.
+    - Case "NNRSEither"%string.
+      destruct sf as [disjc [disjd [nin1Δc [nin1Δd [nin2Δc [nin2Δd [sf1 sf2]]]]]]].
+      econstructor.
+      + prove_expr_f_t.
+      + specialize (IHs1 ((v, Some τl) :: Γ)); unfold concat_tenvs in *.
+         simpl in IHs1; eauto.
+      + specialize (IHs2 ((v0, Some τr) :: Γ)); unfold concat_tenvs in *.
+         simpl in IHs2; eauto.
+  Qed.
+
+  Theorem tnnrs_to_nnrs_imp_correct_f {Γc} {si:nnrs} {τ} :
+    [ Γc ⊢ si ▷ τ ]%nnrs_scope ->
+    nnrs_cross_shadow_free si ->
+    [ Γc ⊢ nnrs_to_nnrs_imp si ▷ τ ]%nnrs_imp_scope.
+  Proof.
+    destruct si; simpl.
+    intros typ sf.
+    apply tnnrs_stmt_to_nnrs_imp_correct_f in typ; eauto.
+    split.
+    - unfold nnrs_cross_shadow_free in sf; simpl in sf.
+      apply nnrs_stmt_to_nnrs_imp_stmt_not_used_without_assignment.
+      + apply nnrs_stmt_cross_shadow_free_under_free_env_mdenv in sf.
+         apply disjoint_cons_inv2 in sf; tauto.
+      + apply nnrs_stmt_cross_shadow_free_under_free_mcenv_mdenv in sf.
+        apply disjoint_cons_inv2 in sf; tauto.
+    - unfold concat_tenvs in typ; simpl in typ; trivial.
+  Qed.
+  
+  Theorem tnnrs_to_nnrs_imp_top_correct_f {Γc} {si:nnrs} {τ} :
+    [ Γc ⊢ si ▷ τ ]%nnrs_scope ->
+    forall sep,
+      [ Γc ⊢ nnrs_to_nnrs_imp_top sep si ▷ τ ]%nnrs_imp_scope.
+  Proof.
+    intros typ sep.
+    apply tnnrs_to_nnrs_imp_correct_f.
+    - apply nnrs_uncross_shadow_type; trivial.
+    - apply nnrs_uncross_shadow_free.
+  Qed.
+
+  Lemma nnrs_stmt_to_nnrs_imp_stmt_assigned_must_assign {s v} :
+    nnrs_imp_stmt_var_usage (nnrs_stmt_to_nnrs_imp_stmt s) v = VarMustBeAssigned ->
+    nnrs_stmt_must_assign s v.
+  Proof.
+    nnrs_stmt_cases (induction s) Case
+    ; simpl; intros eqq
+    ; try solve [repeat match_destr_in eqq; try tauto].
+    - Case "NNRSLetMut"%string.
+      unfold equiv_decb in *.
+      destruct (v0 == v); try discriminate.
+      match_destr_in eqq; tauto.
+    - Case "NNRSAssign"%string.
+      unfold equiv_decb in *.
+      destruct (v0 == v); try discriminate.
+      match_destr_in eqq; tauto.
+      match_destr_in eqq; tauto.
+    - Case "NNRSPush"%string.
+      unfold equiv_decb in eqq.
+      destruct (v0 == v)
+      ; destruct (v == v0)
+      ; simpl in eqq
+      ; try congruence.
+      match_destr_in eqq.
+  Qed.
+    
+  Section core.
+
+    Program Theorem tnnrs_core_to_nnrs_imp_core_top_correct_f {Γc} {si:nnrs_core} {τ} :
+      [ Γc ⊢ si ▷ τ ]%nnrs_scope ->
+      forall sep,
+        [ Γc ⊢ nnrs_core_to_nnrs_imp_core_top sep si ▷ τ ]%nnrs_imp_scope.
+    Proof.
+      intros typ sep.
+      apply tnnrs_to_nnrs_imp_top_correct_f; trivial.
+    Qed.
+      
+  End core.
+
+End TNNRStoNNRSimp.
